src/cardinality/propagate.lean
@@ -1,0 +1,137 @@
+/-
+
+Experiments with propagation structures.
+
+Author: Cayden Codel
+-/
+
+import data.list.basic
+import cnf.cnf
+import cnf.gensym
+import cnf.encoding
+import cardinality.distinct
+import cardinality.cardinality
+
+variables {V : Type*} [inhabited V] [decidable_eq V]
+
+namespace propagate
+
+open list
+open literal
+open cnf
+open clause
+open assignment
+open distinct
+open prod
+open gensym
+open encoding
+open amk
+
+def propagate : list (literal V) → cnf V
+| []               := []
+| [l₁]             := []
+| (l₁ :: l₂ :: ls) := [l₁.flip, l₂] :: propagate (l₂ :: ls)
+
+@[simp] theorem propagate_nil : propagate ([] : list (literal V)) = [] := rfl
+
+@[simp] theorem propagate_singleton : ∀ (l : literal V), propagate [l] = [] :=
+assume l, rfl
+
+theorem propagate_truth {τ : assignment V} {l : list (literal V)} {l₁ l₂ : literal V} : 
+  (propagate l).eval τ = tt → distinct l₁ l₂ l → l₁.eval τ = tt → l₂.eval τ = tt :=
+begin
+  intros hp hdis h₁,
+  induction l with x₁ ls ih generalizing l₁,
+  { exact absurd hdis (not_distinct_nil _ _) },
+  { cases ls with x₂ ls,
+    { exact absurd hdis (not_distinct_singleton _ _ _) },
+    { cases ls with x₃ ls,
+      { rcases eq_of_distinct_double hdis with ⟨rfl, rfl⟩,
+        simp [propagate, clause.eval_cons, eval_flip, h₁] at hp,
+        exact hp },
+      { rw propagate at hp,
+        simp [cnf.eval_cons] at hp,
+        rcases hp with ⟨hp₁, hp₂⟩,
+        rcases eq_or_distinct_of_distinct_cons hdis with (rfl | h),
+        { simp [clause.eval_cons, eval_flip, h₁] at hp₁,
+          rcases eq_or_mem_of_mem_cons (mem_tail_of_distinct_cons hdis)
+            with (rfl | h₂),
+          { exact hp₁ },
+          { exact ih hp₂ (distinct_cons_of_mem x₂ h₂) hp₁ } },
+        { exact ih hp₂ h h₁ } } } }
+end
+
+def zipped_propagate (l : list (list (literal V) × literal V)) : cnf V :=
+l.map (λ p, ((fst p).map (literal.flip)) ++ [snd p])
+
+theorem zipped_propagate_truth {τ : assignment V} 
+  {l : list (list (literal V) × literal V)} :
+  (zipped_propagate l).eval τ = tt ↔ 
+  (∀ p ∈ l, ((∀ (lit : literal V), lit ∈ (fst p) → lit.eval τ = tt) → (snd p).eval τ = tt)) :=
+begin
+  induction l with l ls ih,
+  { simp [zipped_propagate] },
+  { sorry }
+end
+
+def sinz_amkv2 (k : nat) {g : gensym V} {l : list (literal V)} 
+  (hdis : disjoint g.stock (clause.vars l)) (hnil : l ≠ []) : cnf V :=
+
+-- A (k + 1) x n matrix where the (i, j) is s_{i, j} corresponding to x_i and counter (j + 1)
+--
+let S : (nat → nat → V) := λ r c, g.nth ((r * length l) + c) in
+
+-- A single unit clause for the (k + 1)th counter variable for x_n
+[Neg (S k (length l))] ::
+
+-- For each of the (k + 1) rows, take the row and encode propagation forward
+-- Flatten the propagate results for each row
+(foldl (λ l₁ l₂, l₁ ++ l₂) ([] : cnf V) 
+  -- Take each row (k + 1 rows, each with length n)
+  ((range (k + 1)).map (λ i, 
+    -- Generate clauses that propagate truth of same counter signal variables
+    propagate ((range (length l)).map (λ j, Pos (S i j)))))) ++
+
+-- Take each x_i and make x_i => s_{i, 1}
+l.map_with_index (λ i x, [x.flip, Pos (S 0 i)]) ++
+
+-- For each signal variable not on the first row or column, 
+-- make (x_{i} ^ s_{i - 1, j - 1} => s_{i, j})
+(foldl (λ l₁ l₂, l₁ ++ l₂) ([] : cnf V) 
+  (l.tail.map_with_index (λ i x, 
+    (range k).map (λ j, 
+      [x.flip, Neg (S j i), Pos (S (j + 1) (i + 1))]))))
+
+theorem enc (k : nat) {g : gensym V} {l : list (literal V)}
+  (hdis : disjoint g.stock (clause.vars l)) (hnil : l ≠ []) : 
+  encodes (amk k) (sinz_amkv2 k hdis hnil) l :=
+begin
+  intro τ,
+  induction k with k ih,
+  split,
+  { intro hamk,
+    use assignment.ite (clause.vars l) τ all_ff,
+    split,
+    { 
+      rw sinz_amkv2,
+      rw eval_tt_iff_forall_clause_eval_tt,
+      simp,
+      split,
+      { have := set.disjoint_left.mp hdis (nth_mem_stock g l.length),
+        rw [literal.eval, ite_neg this, all_ff_eval_ff],
+        refl },
+      {
+        intros c hc,
+        rcases hc with (hc | hc | hc),
+        { simp [range, range_core] at hc,
+          sorry -- by facts of propogate, can always find one!
+        },
+        {
+          
+        }
+      }
+    },
+    { exact (ite_eqod (clause.vars l) τ all_ff).symm } }
+end
+
+end propagate
